concur/CallConvLibs.v
@@ -1,0 +1,383 @@
+Require Import LanguageInterface CallconvAlgebra Invariant.
+Require Import CKLR Inject InjectFootprint Extends.
+Require Import Mach Locations Conventions Asm.
+Require Import ValueAnalysis.
+Require Import Allocproof Lineartyping Asmgenproof0.
+Require Import Maps Stacklayout.
+
+Require Import CallconvBig VCompBig.
+Require Import StackingproofC CallConv.
+Import GS.
+
+Section TRANS.
+
+  Context {li1 li2} (cc : LanguageInterface.callconv li1 li2).
+  Variable L1 : semantics li1 li1.
+  Variable L2 : semantics li2 li2.
+
+  Hypothesis OLDSIM: Smallstep.forward_simulation cc cc L1 L2.
+
+  Lemma NEWSIM: GS.forward_simulation cc L1 L2.
+  Proof.
+    intros. inv OLDSIM. constructor.
+    inv X. econstructor; eauto.
+    intros. exploit fsim_lts0; eauto.
+    intros FPros.
+    instantiate (1:= fun se1 se2 wB gw idx s1 s2 =>  fsim_match_states0 se1 se2 wB idx s1 s2).
+    simpl.
+    inv FPros. econstructor; eauto.
+    - intros. exploit fsim_match_final_states0; eauto.
+      intros [r2 [A B]]. exists r2. exists tt. intuition auto. reflexivity. reflexivity.
+    - intros. exploit fsim_match_external0; eauto.
+    intros (w0 & q2 & A & B & C).
+    exists w0, q2. intuition auto. reflexivity.
+    eapply H4; eauto.
+  Qed.
+
+End TRANS.
+(*    
+Program Definition cc_id {li : language_interface} : callconv li li :=
+  {|
+    ccworld := unit;
+    ccworld_world := world_unit;
+    match_senv w := eq;
+    match_query w := eq;
+    match_reply w := eq;
+  |}.
+ *)
+
+Lemma cctrans_id_1 {li1 li2 : language_interface} : forall (cc: callconv li1 li2),
+    cctrans (cc_compose cc_id cc) cc.
+Proof.
+  econstructor. instantiate (1:= fun w1 w => eq (snd w1) w).
+  - econstructor. repeat apply conj; eauto.
+    + instantiate (1:= (se1,(tt,w2))). econstructor; eauto. reflexivity.
+    + econstructor; eauto. split. reflexivity. auto.
+    + reflexivity.
+    + intros. destruct wp1 as [xx wp2']. simpl in H1, H2.  subst wp2'.
+      destruct wp1' as [xy wp2'']. destruct H3. destruct H2. simpl in *.
+      eexists. split; eauto. split; eauto.
+      destruct H4 as [r1' [A B]]. subst. auto.
+  - red. intros. destruct w1 as [se' [tt w2]].
+    simpl in H. destruct H as [Heq H]. subst se'.
+    simpl in H0. destruct H0 as [q1' [Heq H0]]. subst q1'.
+    destruct wp1 as [tt' wp2'].
+    destruct H1. simpl in H1, H3. simpl in H2. subst wp2'.
+    exists w2. intuition auto.
+    exists (tt, wp2'). intuition auto.
+    split; auto. exists r1. split. econstructor; eauto. auto.
+Qed.
+
+Lemma cctrans_id_2 {li1 li2 : language_interface} : forall (cc: callconv li1 li2),
+    cctrans (cc_compose cc cc_id) cc.
+Proof.
+  econstructor. instantiate (1:= fun w1 w => eq (fst w1) w).
+  - econstructor. repeat apply conj; eauto.
+    + instantiate (1:= (se2,(w2,tt))). econstructor; eauto. reflexivity.
+    + exists q2. split; auto. econstructor; eauto.
+    + reflexivity.
+    + intros. destruct wp1 as [wp2' xx]. simpl in H1, H2.  subst wp2'.
+      destruct wp1' as [wp2'' xy]. destruct H3. destruct H2. simpl in *.
+      eexists. split; eauto. split; eauto.
+      destruct H4 as [r1' [A B]]. subst. auto.
+  - red. intros. destruct w1 as [se' [w2 tt]].
+    simpl in H. destruct H as [H Heq]. subst se'.
+    simpl in H0. destruct H0 as [q2' [H0 Heq]]. subst q2'.
+    destruct wp1 as [wp2' tt'].
+    destruct H1. simpl in H1, H3. simpl in H2. subst wp2'.
+    exists w2. intuition auto.
+    exists (wp2',tt). intuition auto. split; simpl. auto. reflexivity.
+    exists r2. split. auto. econstructor; eauto.
+Qed.
+
+Lemma oldfsim_newfsim_ccid : forall {li : language_interface} (L1 L2: semantics li li),
+    Smallstep.forward_simulation LanguageInterface.cc_id LanguageInterface.cc_id L1 L2 ->
+    forward_simulation cc_id L1 L2.
+Proof.
+  intros. generalize (NEWSIM LanguageInterface.cc_id L1 L2).
+  intro. apply H0. auto.
+Qed.
+
+
+(** Q : Can we (Should we) define the new [injp] as [cklr] instead of several different
+        callconvs for different interfaces ?
+      
+    1. Compare the [c_injp] defined above v.s. [cc_c injp]. 
+       Can we define another version of cc_c based on another [cklr] equipped with acci and acce?
+    2. Try []
+
+  *)
+
+Lemma compose_id_new_injp_1 {li1 li2: language_interface} : forall (cc: callconv li1 li2) L1 L2 L3,
+    Smallstep.forward_simulation 1 1 L1 L2 ->
+    forward_simulation cc L2 L3 ->
+    forward_simulation cc L1 L3.
+Proof.
+  intros. eapply open_fsim_cctrans.
+  eapply st_fsim_vcomp; eauto. eapply oldfsim_newfsim_ccid; eauto.
+  eapply cctrans_id_1.
+Qed.
+
+Lemma compose_id_new_injp_2 {li1 li2: language_interface} : forall (cc: callconv li1 li2) L1 L2 L3,
+    forward_simulation cc L1 L2 ->
+    Smallstep.forward_simulation 1 1 L2 L3 ->
+    forward_simulation cc L1 L3.
+Proof.
+  intros. eapply open_fsim_cctrans.
+  eapply st_fsim_vcomp; eauto. eapply oldfsim_newfsim_ccid; eauto.
+  eapply cctrans_id_2.
+Qed.
+
+Require Import Extends.
+
+(** c_ext cannot be defined using cc_unit_world because [cc_c] uses <> diamond constructer for match_reply*)
+Program Definition c_ext : callconv li_c li_c := cc_c ext.
+(*  {|
+    ccworld := unit;
+    ccworld_world := world_unit;
+    match_senv w := eq;
+    match_query w := cc_c_query ext w;
+    match_reply w := cc_c_reply ext w;
+  |}.
+*)
+Lemma cctrans_ext_comp : cctrans (cc_compose c_ext c_ext) c_ext.
+Proof.
+  econstructor. instantiate (1:= fun _ _ => True).
+  - red. intros. inv H.  inv H0. simpl in H, H1, H2.
+    exists (se2, (tt,tt)). intuition auto. econstructor; eauto. reflexivity. reflexivity.
+    exists (cq vf1 sg vargs1 m1). split.
+    econstructor; eauto. reflexivity. simpl.
+    generalize dependent vargs1.
+    induction 1. constructor. constructor; eauto. reflexivity.
+    simpl. eapply Mem.extends_refl.
+    econstructor; eauto.
+    exists tt. intuition auto. destruct wp1'. simpl in H6. 
+    destruct H6 as [r1' [[? [A0 A]][? [B0 B]]]]. inv A. inv B. simpl in *.
+    exists tt. split. eauto.
+    econstructor; simpl; eauto.
+    eapply val_inject_id. eapply Val.lessdef_trans; eapply val_inject_id; eauto.
+    eapply Mem.extends_extends_compose; eauto.
+  - red. intros. destruct w1 as [se' [w11 w12]]. inv H. inv H3. inv H4. inv H2.
+    inv H0. inv H. inv H0. inv H2. simpl in H9, H11, H12, H , H3, H4.
+    exists tt. intuition auto. reflexivity. constructor.
+    constructor; simpl; eauto.
+    eapply val_inject_id. eapply Val.lessdef_trans; eapply val_inject_id; eauto.
+    eapply CallConv.val_inject_lessdef_list_compose. eauto.
+    eapply (ext_lessdef_list tt). eauto.
+    eapply Mem.extends_extends_compose; eauto.
+    exists (tt,tt). split. reflexivity. split. exists r1. destruct H2 as [? [X H2]]. inv H2. simpl in *.
+    split. exists tt. split. eauto.
+    econstructor; simpl; eauto. eapply val_inject_id.
+    eapply Val.lessdef_refl.
+    eapply Mem.extends_refl.
+    exists tt. split. eauto.
+    econstructor; eauto. auto.
+Qed.
+
+
+Lemma oldfsim_newfsim_ext_c : forall  (L1 L2: semantics li_c li_c),
+    Smallstep.forward_simulation (cc_c ext) (cc_c ext) L1 L2 ->
+    forward_simulation c_ext L1 L2.
+Proof.
+  intros. red in H. inv H. constructor.
+  inv X. econstructor; eauto.
+  intros. exploit fsim_lts0; eauto.
+  intros FPros.
+  instantiate (1:= fun se1 se2 wB gw idx s1 s2 =>  fsim_match_states0 se1 se2 wB idx s1 s2).
+  simpl.
+  inv FPros. econstructor; eauto.
+  - intros. exploit fsim_match_final_states0; eauto.
+    intros [r2 [A B]]. exists r2. exists tt. intuition auto. reflexivity. reflexivity.
+  - intros. exploit fsim_match_external0; eauto.
+    intros (w0 & q2 & A & B & C).
+    exists w0, q2. intuition auto. reflexivity.
+    eapply H4; eauto.
+Qed.
+
+
+(** Big Problem : bring lower cklrs to C level *)
+
+Program Instance lens_injp_locset : Lens (signature * injp_world) injp_world :=
+  {
+    get := snd;
+    set := fun w wp => (fst w, wp);
+  }.
+
+Program Instance injp_world_id_l : World (signature * injp_world) :=
+    {
+      w_state := injp_world;
+      w_lens := lens_injp_locset;
+      w_acci := injp_acci;
+      w_acce := injp_acce;
+      w_acci_trans := injp_acci_preo;
+    }.
+(* cc_locset *)
+Program Definition locset_injp : callconv li_locset li_locset :=
+  {|
+    ccworld := signature * injp_world;
+    ccworld_world := injp_world_id_l;
+    match_senv w := CKLR.match_stbls injp (snd w);
+    match_query w := cc_locset_query injp (fst w) (snd w);
+    match_reply w := cc_locset_reply injp (fst w) (snd w);    
+  |}.
+Next Obligation.
+  inv H. inv H0. auto.
+Qed.
+Next Obligation.
+  intros. inv H. erewrite <- Genv.valid_for_match; eauto.
+Qed.
+
+Infix "@" := GS.cc_compose (at level 30, right associativity).
+
+Inductive match12_stacking : injp_world -> (injp_world * unit) -> Prop :=
+|match12_stacking_intro : forall f m1 m2 Hm Hm' t,
+    match12_stacking (injpw f m1 m2 Hm) ((injpw f m1 m2 Hm'),t).
+
+Lemma Asmtrans : cctrans (cc_stacking_injp) (locset_injp @ cc_locset_mach).
+Proof.
+  simpl. econstructor. instantiate (1:= match12_stacking).
+  - red. intros w2 se1 se2 q1 q2 Hse Hq.
+    destruct w2 as [se [[sig wx] [sig' rs]]].
+    destruct Hse as [Hse1 Hse2]. simpl in Hse1, Hse2. inv Hse2.
+    destruct Hq as [q1' [Hq1 Hq2]]. inv Hq2. simpl in Hq1. inv Hq1.
+    inv H9. simpl in H4, Hse1, H8.
+    set (rs2 := (make_locset rs lmw_m lmw_sp)).
+    inv H5.
+    + (*no stack-allocated arguments *)
+      red in H.
+    exists (stkw injp (injpw f m1 m_ Hm) sig' ls1 lmw_sp m_).
+    repeat apply conj; eauto.
+    -- econstructor; eauto. admit. (*to de added in LM*)
+       intros. apply H8. constructor. constructor; eauto with mem.
+       split. intro. extlia. intros. exfalso. admit.
+       intros. rewrite H in H0. inv H0. extlia.
+    -- simpl. constructor.
+    -- intros. inv H0. simpl in H1, H3.
+       exists (wp1', tt). simpl. repeat apply conj; eauto.
+       simpl.  inv H1. constructor; eauto.
+       simpl. inv H2. constructor; eauto.
+       inv H3.
+       set (ls2' := make_locset rs2' m2' lmw_sp).
+       exists (lr ls2' m2'). split.
+       constructor; eauto. constructor.
+       constructor; eauto.
+
+       red in H8.
+       intros. specialize (H8 (R r)) as HH.
+       exploit HH. constructor.
+       intro VINJ1.
+       exploit H16. eauto. intro VINJ2. simpl in VINJ1.
+       admit. (** need fix, about callee-save regs *)
+       eauto with mem.
+       intros. rewrite H in H0. inv H0. extlia.
+    +
+     assert (Hm' : Mem.inject f m1 lmw_m). admit. simpl in Hse1.
+     exists (stkw injp (injpw f m1 lmw_m Hm') sig' ls1 (Vptr sb sofs) lmw_m).
+     repeat apply conj; eauto.
+     -- inv Hse1. constructor; eauto. erewrite <- Mem.support_free; eauto.
+     -- econstructor; eauto. admit. (*to de added in LM*)
+       intros. apply H8. constructor. constructor; eauto with mem.
+       split. intros. do 2 eexists. split. reflexivity. split.
+       eapply Mem.free_range_perm. eauto. eauto.
+       intros. exploit H2; eauto. intros [v Hv]. exists v. split. auto.
+       exploit H8. eapply loc_external_arg. eauto.
+       simpl. setoid_rewrite Hv. simpl. auto.
+       intros. red. intros. inv H3.
+       intro. exploit Mem.perm_inject. eauto. apply Hm1. eauto.
+       replace (ofs - delta + delta) with ofs by lia.
+       intros.
+       eapply Mem.perm_free_2; eauto. 
+    -- simpl. admit. (** match should contain [args_removed] *)
+    -- intros. inv H3. simpl in H5, H11.
+       exists (wp1', tt). simpl. repeat apply conj; eauto.
+       simpl. inv H5. constructor; eauto.
+       simpl. inv H11. constructor; eauto.
+       inv H3.
+       set (ls2' := make_locset rs2' m2' lmw_sp).
+       exists (lr ls2' m2'). split.
+       constructor; eauto. constructor.
+       constructor; eauto.
+
+       red in H8.
+       intros. specialize (H8 (R r)) as HH.
+       exploit HH. constructor.
+       intro VINJ1.
+       exploit H16. eauto. intro VINJ2. simpl in VINJ1.
+       admit. (** need fix, about callee-save regs *)
+       eauto with mem.
+       intros. rewrite H in H0. inv H0. extlia.
+      intros. inv H0. simpl in H1, H3.
+       exists (wp1', tt). simpl. repeat apply conj; eauto.
+       simpl.  inv H1. constructor; eauto.
+       simpl. inv H2. constructor; eauto.
+       inv H3.
+       set (ls2' := make_locset rs2' m2' lmw_sp).
+       exists (lr ls2' m2'). split.
+       constructor; eauto. constructor.
+       constructor; eauto.
+
+       red in H8.
+       intros. specialize (H8 (R r)) as HH.
+       exploit HH. constructor.
+       intro VINJ1.
+       exploit H16. eauto. intro VINJ2. simpl in VINJ1.
+       admit. (** need fix, about callee-save regs *)
+       eauto with mem.
+       intros. rewrite H in H0. inv H0. extlia.
+
+
+      admit. (** same but more complicated *)
+  - red. intros. simpl in wp1, wp2, w1.
+    inv H0. inv H. cbn in H1. inv H2.
+    Compute ccworld (locset_injp @ cc_locset_mach).
+    exists (se2, (sg, (injpw f m1 m2 Hm), (lmw sg rs2 m2 sp2))).
+    repeat apply conj; simpl; eauto.
+    + inv H1. constructor; eauto.
+    + set (ls2 := make_locset rs2 m2 sp2).
+      exists (lq vf2 sg ls2 m2). split.
+      constructor; eauto. red. intros; simpl; eauto.
+      inv H. eauto. inv H6. admit.
+      constructor.
+      constructor; eauto. admit.
+    + 
+        
+
+      
+
+  intros.
+
+
+
+
+(** Idea: first try to compose all C level passes? Clight -> LTL *)
+
+(** Idea: Since we have totally the same incoming and outgoing lemmas. The [inj] is useless? *)
+(* inj *)
+(*
+Local Instance world_inj : World inj_world :=
+  {
+    w_state := inj_world;
+    w_lens := lens_id;
+    w_acci := inj_incr;
+    w_acce := inj_incr;
+  }.
+
+Program Definition c_inj : callconv li_c li_c :=
+  {|
+    ccworld := inj_world;
+    ccworld_world := world_inj;
+    match_senv w := inj_stbls w;
+    match_query w := cc_c_query inj w;
+    match_reply w := cc_c_reply inj w;
+  |}.
+
+*)
+
+(** 4.1 The self-simulation mechniasm? *)  
+(** 4.Modify the proofs of each pass *)
+(** 5.Compose the compiler *)
+
+  
+
+
+(** *)
