Makefile
@@ -200,7 +200,7 @@ CLOSE=SmallstepClosed.v
 CONCUR=MultiLibs.v CMulti.v AsmMulti.v \
        CallconvBig.v MultiSimBig.v \
        HCompBig.v \
-       InjpAccoComp.v VCompBig.v \
+       InjpAccoComp.v VCompBig.v CallConvLibs.v \
        SimplLocalsproofC.v CminorgenproofC.v InliningproofC.v \
        InvariantC.v StackingproofC.v \
        ConstpropproofC.v CSEproofC.v DeadcodeproofC.v UnusedglobproofC.v \
